Consider the motion of a body $m$ orbiting circularly around a much more massive body $M$. The [[Gravitational Potential Energy]] of the system is:
$$
U(r)=-\frac{GMm}{r}
$$
The [[Kinetic Energy]] of the system is:
$$
K=\frac{1}{2}mv^2=\frac{1}{2}m\omega^2r^2
$$
as $M$ is considered to be at rest. By making [[Newton's Law of Gravitation]] equivalent to [[Centripetal Force]]:
$$
\begin{align}
\frac{GMm}{r^2}&=m \frac{v^2}{r} \\
\frac{GM}{r}&=v^2 \\
\frac{GM}{r}&=\omega^2 r^2
\end{align}
$$
We can substitute this with Kinetic Energy:
$$
K=\frac{GMm}{2r}
$$
So the total [[Mechanical Energy]] is:
$$
E=K+U=\frac{GMm}{2r}- \frac{GMm}{r} = \boxed{-\frac{GMm}{2r}}
$$
The equation above is still valid for elliptical orbits when we replace $r$ with the semimajor axis $a$.

The interpretation of this constant and negative energy is that the system is closed, and $m$ is always bound to $M$. For $m$ to escape $M$, it would need a positive energy as $a$ tends towards infinity. However, both $K$ and $U$ tend towards 0. If we supply enough energy so that it is positive or 0, then the orbit is no longer elliptical. When $E=0$, it is parabolic, and when $E>0$, it is hyperbolic.

The equation also tells us that we cannot change the speed without changing the radius. If we want to increase the speed of a satellite, it increasing kinetic energy. As a result the total energy is less negative and the radius increases.